


\chapter{Proof Continued for \texorpdfstring{\(\gamma \leq 0\)}{gamma <= 0}}\label{chapter:proof-gamma-negative}

The main idea of the proof for \(\gamma > 0\) was that \(f_n\) converges to some reconstruction \(f = \mathcal{R}f\) if \(\gamma > 0\), where \(f_n = f_1 + \sum\limits^{n-1}_{k=1} g_k'  + \sum\limits^{n-1}_{k=1} g_k''\), see~\eqref{approximating-distributions-alternative}.   
If however \(\gamma \leq 0\), the series \(\sum g_k''(\psi)\) need not converge. We fix this by ignoring \(\sum g_k''(\psi)\); the approximating distribution then reads \(f_1 + \sum\limits^{n-1}_{k=1} g_k'(\psi)\). We set 
\begin{align*}
    f^K(\psi) = f_1(\psi) + \lim_{n\to \infty}\sum^{n-1}_{k=1} g_k'(\psi),
\end{align*}
which is well-defined because \(\sum g_k'(\psi)\) converges for all \(\gamma \in \mathbb{R}\) (see Chapter~\ref{chapter:step-3}). Next, \(f^K\) is a distribution on \(\bar K_1\) because TO-DO

In the next steps, we will show that \(f^K\) satisfies~\eqref{reconstruction-theorem}, i.e.
\begin{gather*}
    |(f^K - F_x)(\psi_x^\lambda)| \leq \mathfrak{C} \vertiii{F}^{\mathrm{coh}}_{\bar K_{2},\varphi,\alpha,\gamma} \begin{cases}
        \lambda^\gamma  &\text{if \(\gamma < 0\)}\\
        1 + |\log(\lambda)| \quad &\text{if \(\gamma = 0\) } 
    \end{cases}
    \\
    \text{uniformly for \(\psi \in \mathcal{B}_r\), \(x \in K\) and \(\lambda \in(0,1]\).   }
\end{gather*}
where the constant \(\mathfrak{C}\) is given by TO-DO and TO-Do. We will then spend another chapter to build a \emph{global} distribution \(f \in \mathcal{D}'\) out of the local distributions \(f^K \in \mathcal{D}(\bar K_1)\) such that \(f\) satisfies~\eqref{reconstruction-theorem}, as well.

\section{Step 5: \texorpdfstring{\(f^K\) is a local reconstruction}{fK is a local reconstruction}}
 
We have the same setup as in Chapter~\ref{setup}: Step 0. Let \(K \subset \mathbb{R}^d\) be a compact set, \(x \in K\), \(\psi \in \mathcal{B}_r\) and \(\lambda \in (0,1]\). Then, we have
\begin{align*}
    |(f^K - F_x)(\psi_x^\lambda)|
    &= |((f_1 + \lim_{n\to \infty}\sum_{k=1}^{n-1}g_k') - F_x)(\psi_x^\lambda)| \\
    &= |(f_1 + \lim_{n\to \infty}\sum_{k=1}^{n-1}g_k')(\psi_x^\lambda) - \lim_{n\to \infty} F_x(\psi_x^\lambda* \rho^{\epsilon_n})| \\
    &= \lim_{n \to \infty} |\underbrace{f_1(\psi_x^\lambda) + \left\{ \sum_{k=1}^{n-1}g_k'(\psi_x^\lambda) \right\} - F_x(\psi_x^\lambda* \rho^{\epsilon_n})}_{\coloneqq \bar f_n(\psi_x^\lambda)}|.
\end{align*}  
Next, we write the above expression as a telescopic sum 
\begin{align*}
    |(f^K - F_x)(\psi_x^\lambda)| = 
    \lim_{n \to \infty} |\bar f_n(\psi_x^\lambda)| \leq 
    | \left ( \lim_{n \to \infty} \bar f_n(\psi_x^\lambda) \right ) - \bar f_N(\psi_x^\lambda)|
    + |\bar f_N(\psi_x^\lambda)|
\end{align*}
where \(N\) is chosen such that \(\epsilon_N \leq \lambda < \epsilon_{N - 1}\). The first summand is estimated by Lemma~\ref{technical-lemma-2}
\begin{align*}
    | \left( \lim_{n \to \infty} \bar f_n(\psi_x^\lambda)  \right) - \bar f_N(\psi_x^\lambda)| &\leq
    \sum_{k \geq N} |(\bar f_{k+1} - \bar f_{k})(\psi_x^\lambda)|\\ &= 
    \sum_{k \geq N} |g_k'(\psi^\lambda_x) - F_x(\psi^\lambda_x*(\rho^{\epsilon_{k+1}}-\rho^{\epsilon_k}))| \\
    &\Downarrow \text{Lemma~\ref{technical-lemma-2}} \\
    &\leq \left \{ \frac{\hat C 4^{\gamma - \alpha + d} \lVert \check \varphi \rVert_{L^1} }{1-2^{-\alpha - r}} \right \} \lambda^{\gamma}.
\end{align*}
The second summand \(|\bar f_N(\psi_x^\lambda)|\) is also bounded by Lemma~\ref{technical-lemma-2}
\begin{align*}
    |\bar f_N(\psi_x^\lambda)| &\leq |\bar f_1(\psi_x^\lambda)| + \sum^{N-1}_{k=1} |(\bar f_{k+1}  - \bar f_k)(\psi_x^\lambda)|\\
    &= |\bar f_1(\psi_x^\lambda)| + \sum^{N-1}_{k=1} |g_k'(\psi^\lambda_x) - F_x(\psi^\lambda_x*(\rho^{\epsilon_{k+1}}-\rho^{\epsilon_k}))| \\
    &\Downarrow \parbox{25em}{Lemma~\ref{technical-lemma-2} (use the case \(\epsilon_k \geq \epsilon_{N-1} > \lambda\))}\\
    &\leq  |\bar f_1(\psi_x^\lambda)| + \sum^{N-1}_{k=1} 4^{d+\gamma-\alpha}\hat C \lVert \check \varphi \rVert_{L^1} \epsilon^\gamma_k.
\end{align*}
Next, we observe
\begin{align*}
    |\bar f_1(\psi_x^\lambda)| &= |f_1(\psi_x^\lambda) - F_x(\psi_x^\lambda* \rho^{\epsilon_1})| \\
    &\Downarrow \text{use~\eqref{lemma:mollified-distribution}} \\
    &= \left | \int_{\mathbb{R}^d} F_z(\rho_z^{\epsilon_1}) \psi^\lambda_x(z)  \mathrm{d}z -  \int F_x(\rho_z^{\epsilon_1}) \psi^\lambda_x(z) \mathrm{d} z \right| \\
    &= \left | \int_{\mathbb{R}^d} (F_z - F_x)(\rho_z^{\epsilon_1}) \psi^\lambda_x(z)  \mathrm{d}z\right| \\
    &\Downarrow  \text{Recall \(\rho = \hat \varphi^2 * \hat \varphi\) and use~\eqref{lemma:mollified-distribution}} \\
    &= \left| \iint (F_z - F_x)(\hat \varphi^{\epsilon_1}_y) \hat \varphi^{2\epsilon_1}(y-z)\psi^\lambda_x(z) \; \mathrm{d}y \, \mathrm{d}z \right|.
\end{align*}
The tweaked test function \(\hat \varphi\) has a compact support in \(B(0, \frac{1}{2})\); hence \(\hat \varphi^{2\epsilon}\) is supported in \(B(0, \epsilon_1)\). Thus, the integral is nonzero if \(|y-z| \leq \epsilon_1 = \frac{1}{2}\). Additionally, we have \(|x-z|\leq \lambda\) because \(\psi^\lambda_x(z)\). So, we estimate
\begin{align*}
    |\bar f_1(\psi_x^\lambda)| &\leq  \sup_{\substack{z \in B(x, \lambda) \\ |y-z| \leq \frac{1}{2}}} \left| (F_z - F_x)(\hat \varphi^{\epsilon_1}_y) \right|  \cdot \lVert \hat \varphi^{2\epsilon_1} \rVert_{L^1} \lVert  \psi^{\lambda}_x \rVert_{L^1}.
\end{align*}
Moreover, \(z \in \bar K_1\) (recall that \(x \in K\) and \(\lambda \in (0,1]\)), \(y \in \bar K_{\frac{3}{2}}\) and \(|x-y| \leq |x-z| + |z-y| \leq \frac{3}{2}\). Hence, we use the triangle inequality and the coherence condition to obtain 
\begin{align*}
    \sup_{\substack{z \in B(x, \lambda) \\ |y-z| \leq
     \frac{1}{2}}} \left| (F_z - F_x)(\hat \varphi^{\epsilon_1}_y) \right| 
     &\leq \sup_{\substack{y, z \in \bar K_{3/2} \\ |y-z| \leq \frac{1}{2}}} \left| (F_z - F_y)(\hat \varphi^{\epsilon_1}_y) \right| + \sup_{\substack{x,y \in \bar K_{3/2} \\ |x-y| \leq \frac{3}{2}}} \left| (F_y - F_x)(\hat \varphi^{\epsilon_1}_y) \right| \\
     &\overset{\eqref{coherence-hat}}{\leq} \hat C \epsilon_1^\alpha(|z-y| + \epsilon_1)^{\gamma - \alpha} + \hat C \epsilon_1^\alpha(|y-x| + \epsilon_1)^{\gamma - \alpha}\\
     &\leq \hat C \left(\frac{3}{2}\right)^{\gamma - \alpha } + \hat C \left(\frac{5}{2}\right)^{\gamma - \alpha } \\
     &\leq 2\hat C \cdot  3^{\gamma - \alpha}.
\end{align*}
We bound
\begin{align*}
    |\bar f_1(\psi_x^\lambda)| \leq \left\{ 2\hat C \cdot  3^{\gamma - \alpha} \right\} \lVert \hat \varphi^{2\epsilon_1} \rVert_{L^1} \lVert  \psi^{\lambda}_x \rVert_{L^1} &= \left\{ 2\hat C \cdot  3^{\gamma - \alpha} \right\} \lVert \hat \varphi \rVert_{L^1} \lVert  \psi \rVert_{L^1} \\
    &\leq \left\{ 2\hat C \cdot  3^{\gamma - \alpha} \right\}  \lVert \hat \varphi \rVert_{L^1} \cdot \sup_{\psi \in \mathcal{B}_r} \lVert  \psi \rVert_{L^1} \\
    &\leq \left\{ 2\hat C \cdot  3^{\gamma - \alpha} \right\}  \lVert \hat \varphi \rVert_{L^1} \cdot 2^d \cdot \underbrace{\sup_{\psi \in \mathcal{B}_r} \lVert  \psi \rVert_{\infty}}_{\leq 1} \\
    &\leq 2^{d+1}\hat C \cdot  3^{\gamma - \alpha}  \lVert \hat \varphi \rVert_{L^1}.
\end{align*}
Then, we have \(|\bar f_N(\psi_x^\lambda)| \leq 2^{d+1}\hat C \cdot  3^{\gamma - \alpha}  \lVert \hat \varphi \rVert_{L^1} + \sum^{N-1}_{k=1} 4^{d+\gamma-\alpha}\hat C \lVert \check \varphi \rVert_{L^1} \epsilon^\gamma_k\). Also observe that 
\(\lVert \check \varphi \rVert_{L^1} = \int |\check \varphi(x)| \mathrm{d}x \leq \int|\hat \varphi^{\frac{1}{2}}(x)| + |\hat \varphi^{2}(x)| \mathrm{d}x = 2\int |\hat \varphi(x)| \mathrm{d}x = 2 \lVert \hat \varphi \rVert_{L^1}\). So, we get 
\begin{align*}
|\bar f_N(\psi_x^\lambda)| \leq 4^{d + \gamma - \alpha + 1} \hat C \lVert \hat \varphi \rVert_{L^1} \sum^{N-1}_{k=0}\epsilon^\gamma_k.
\end{align*}
Note that \(\sum^{N-1}_{k=0}\epsilon^\gamma_k\) is a geometric sum which we explicitly compute
\begin{align*}
    \sum^{N-1}_{k=0}\epsilon^\gamma_k = 
    \sum^{N-1}_{k=0}2^{-\gamma k} \leq \begin{dcases}
        \frac{\lambda^\gamma}{1-2^\gamma} \quad &\text{if \(\gamma < 0\) } \\
        \frac{\log(\frac{2}{\lambda})}{\log 2} &\text{if \(\gamma = 0\) }
    \end{dcases}.
\end{align*} 
Finally,
\begin{align*}
    |(f^K - F_x)(\psi_x^\lambda)| &\leq  \frac{\hat C 4^{\gamma - \alpha + d} \lVert \check \varphi \rVert_{L^1} }{1-2^{-\alpha - r}} \lambda^{\gamma} + 4^{d + \gamma - \alpha + 1} \hat C \lVert \hat \varphi \rVert_{L^1}\begin{dcases}
        \frac{\lambda^\gamma}{1-2^\gamma} \quad &\text{if \(\gamma < 0\) } \\
        \frac{\log(\frac{2}{\lambda})}{\log 2} &\text{if \(\gamma = 0\) }
    \end{dcases}.
\end{align*}
If \(\gamma < 0\), then 
\begin{align}
    |(f^K - F_x)(\psi_x^\lambda)| &\;\leq \left\{  \hat C\lVert \hat \varphi \rVert_{L^1}  \frac{4^{\gamma - \alpha + d + 1}}{1 - 2^{-\min\left\{ \alpha + r, - \gamma \right\}}} \right\} \lambda^\gamma \nonumber \\
    &\overset{\eqref{chatnorml1}}{\leq} \left\{ 
        \frac{r^2 2^{\alpha(-r-1)} 4^{d+ \gamma -\alpha + 6} \lVert \varphi \rVert_{L^1}}{1-2^{- \min \left\{ \alpha + r, |\gamma| \right\}} (1+R_{\varphi})^\alpha |\int \varphi(x) \, \mathrm{d}x|^2 }
        \vertiii{F}^{\mathrm{coh}}_{\bar K_{3/2}, \varphi, \alpha, \gamma}.
     \right\}
     \lambda^\gamma. \label{MacbookAirGammaNegative}
\end{align} 
Otherwise if \(\gamma = 0\), then we know \(\log(\frac{2}{\lambda}) (\log{2})^{-1} \leq 2(1 + |\log \lambda|)\). Thus
\begin{align*}
    |(f^K - F_x)(\psi_x^\lambda)| \leq \left\{ 
        \frac{r^2 2^{\alpha(-r-1)} 4^{d -\alpha + 6} \lVert \varphi \rVert_{L^1}}{1-2^{- \min \left\{ \alpha + r, |\gamma| \right\}} (1+R_{\varphi})^\alpha |\int \varphi(x) \, \mathrm{d}x|^2 }
        \vertiii{F}^{\mathrm{coh}}_{\bar K_{3/2}, \varphi, \alpha, \gamma}
     \right\}
     (1 + |\log \lambda|).
\end{align*} 
This shows that \(f^K\) is a local reconstruction. 



% ----------------------------------------



\section{Step 6: \texorpdfstring{Localization}{Localization}}\label{chapter:step6gammaNegative}


Similar to the case \(\gamma > 0\), we need to build a global distribution \(f\) from the local reconstructions \(f^K\). For that, we make use of a localization argument. First, we construct a partition of unity. Fix some test function \(\eta \in \mathcal{D}(B(0, \frac{1}{4}))\) such that \(\eta \geq 0\) on \(B(0, \frac{1}{4})\) and \(\eta \geq 1\) on \(B(0, \frac{1}{8})\). Define 
\begin{align*}
    \xi(x) = \frac{\eta(x)}{\sum\limits_{z \in E} \eta_z(x)} \quad \text{ where } E = \frac{1}{4\sqrt{d}} \mathbb{Z}^d.
\end{align*}
Note that \(\xi_y \in \mathcal{D}(B(y, \frac{1}{4}))\) for every \(y \in \mathbb{R}^d\) and \(\sum\limits_{y \in E} \xi_y \equiv 1\). We call \((\xi_y)_{y \in E}\) a \emph{partition of unity subordinated to the cover \(B(y, \frac{1}{4})_{y \in E}\)}. Define \(B_y = B(y, \frac{1}{4})\). Note that \(B_y\) has diameter \(\frac{1}{2}\). The global reconstruction \(f\) is then defined as
\begin{align*}
    f(\psi) = \sum_{y \in E} f^{B_y}(\xi_y \psi), \quad \forall \psi \in \mathcal{D}.
\end{align*}

Now, we show that \(f\) satisfies the Reconstruction Theorem. Fix a compact set \(K \subset \mathbb{R}^d\), and define 
\begin{align}\label{tropicalGeometryie}
    \alpha = \alpha_{\bar K_2}, \quad \beta = \beta_{\bar K_2}, \quad r > \max\left\{ -\alpha_{\bar K_2}, -\beta_{\bar K_2} \right\}.
\end{align}
Let \(\psi \in \mathcal{B}_r\), \(x \in K\) and \(\lambda \in (0,1]\). For \(\gamma < 0\) we have
\begin{align}\label{AbbaHunter}
    |(f-F_x)(\varphi^\lambda_x)| = |\sum_{y \in E} (f^{B_y} - F_x)(\xi_y \varphi^\lambda_x)| \leq \sum_{y \in E} | (f^{B_y} - F_x)(\xi_y \psi^\lambda_x) |.
\end{align} 
To justify the first equality, note that \(F_x(\varphi^\lambda_x) = F_x(\sum_{y \in E} \xi_y \varphi^\lambda_x) = \sum_{y \in E}F_x(\xi_y \varphi^\lambda_x)\) because \(\sum_{y \in E}\xi_y \equiv 1\).

Next, we make sure that we only sum over a finite number of \(y \in E\). Note that \(\xi_y\) has compact support in \(B(y, \frac{1}{4})\) and \(\psi^\lambda_x\) has compact support in \(B(x, \lambda)\). So, \(\xi_y \psi^\lambda_x \not \equiv 0\) only if \(|y-x| \leq |y - z| + |z-x| \leq \frac{1}{4} + \lambda \leq \frac{5}{4}\). There are at most \((2 \cdot \frac{5}{4} \cdot 4 \sqrt{d} + 1)^d \leq (11 \sqrt{d})^d\) many points \(y \in E\) that satisfy this. 

Then, we write 
\begin{align*}
    | (f^{B_y} - F_x)(\xi_y \psi^\lambda_x) | = | (f^{B_y} - F_x)(\zeta_x^\lambda) |
\end{align*}
for \(\zeta(z) = \xi_y(x + \lambda z) \psi(z)\). We would like to apply~\eqref{MacbookAirGammaNegative} for the compact set \(B_y\) and \(\zeta / \lVert \zeta \rVert_{C^r} \in \mathcal{B}_r\). 
Here, we need to be careful about \(\alpha\), \(\beta\) and \(r\) because we must check that~\eqref{MacbookAirGammaNegative} still holds if we choose \(\alpha\), \(\beta\) and \(r\) as in~\eqref{tropicalGeometryie}. 
Let \(\Gamma = \left\{ y_1,\ldots,y_n \right\} \subset \mathbb{R}^d\) such that \(y_i \cap K \not = \emptyset\) for all \(1 \leq i \leq n\). We have \(\bigcup_{y \in \Gamma}B_y \subset \enlarg{K}{\frac{1}{2}}\) because each ball \(B_y\) has diameter \(\frac{1}{2}\). So, the \(\frac{3}{2}\)-enlargement of \(\bigcup_{y \in \Gamma}B_y\) is contained in \(\enlarg{K}{2}\).
By~\eqref{alpha-monotone} and \(\eqref{beta-monotone}\), we know that the maps \(K \mapsto \alpha_K\) and \(K \mapsto \beta_K\) are monotone. So, we have \(\alpha_{\enlarg{K}{2}} \leq \alpha_{\overline{(\bigcup_{y \in \Gamma}B_y)}_{3/2}}\) and \(\beta_{\enlarg{K}{2}} \leq \beta_{\overline{(\bigcup_{y \in \Gamma}B_y)}_{3/2}}\). This, together with Step 5 (\(\gamma > 0\)), shows that~\eqref{MacbookAirGammaNegative} remains true for \(\alpha, \beta\) and \(r\). Applying~\eqref{MacbookAirGammaNegative} then yields
\begin{align*}
    | (f^{B_y} - F_x)(\zeta_x^\lambda) | = | (f^{B_y} - F_x)(\zeta_x^\lambda / \lVert \zeta \rVert_{C^r}) | \lVert \zeta \rVert_{C^r} &\leq \{ \mathrm{constant} \} \cdot \lVert \zeta \rVert_{C^r} \vertiii{F}^{\mathrm{coh}}_{\enlarg{K}{2}, \varphi, \alpha, \gamma} \lambda^\gamma \\
    &\Downarrow \text{Leibniz Rule and \(\sum_{k=0}^r \binom{r}{k} = 2^r\) }\\
    &\leq  2^r \{ \mathrm{constant} \}\lVert \xi \rVert_{C^r} \lVert \psi \rVert_{C^r} \vertiii{F}^{\mathrm{coh}}_{\enlarg{K}{2}, \varphi, \alpha, \gamma} \lambda^\gamma.
\end{align*} 
Continuing the estimate~\eqref{AbbaHunter} 
\begin{align*}
    |(f-F_x)(\varphi^\lambda_x)| &\overset{\eqref{AbbaHunter}}{\leq} \sum_{y \in E} | (f^{B_y} - F_x)(\xi_y \psi^\lambda_x) | \\ 
    &\;\leq \left\{ (11\sqrt{d})^d \left\{ \mathrm{constant} \right\} \lVert \xi \rVert_{C^r}\lVert \psi \rVert_{C^r}\vertiii{F}^{\mathrm{coh}}_{\enlarg{K}{2}, \varphi, \alpha, \gamma} \right\}\lambda^\gamma.
\end{align*}
The constant before \(\lambda^\gamma\)  then reads
\begin{align}\label{holy-molly}
   \left\{ 2^r \lVert \xi \rVert_{C^r} (11 \sqrt d)^d \frac{r^2 2^{-(r+1) \alpha} 4^{d + \gamma - \alpha + 6}}{1-2^{- \min\left\{ \alpha + r, -\gamma \right\}} |\int \varphi(x) \, \mathrm{d}x|^2  (1 + R_\varphi)^{\alpha}} \lVert \varphi \rVert_{L^1} \right\} \quad \text{in the case \(\gamma < 0\) }.
\end{align}
The proof for the case \(\gamma = 0\) is done similarly and gives the constant 
\begin{align}\label{holy-mollyl}
    \left\{ 2^r \lVert \xi \rVert_{C^r} (11 \sqrt d)^d \frac{r^2 2^{-(r+1) \alpha} 4^{d - \alpha + 6}}{1-2^{- \alpha - r} |\int \varphi(x) \, \mathrm{d}x|^2  (1 + R_\varphi)^{\alpha}} \lVert \varphi \rVert_{L^1} \right\} \quad \text{in the case \(\gamma = 0\) }.
\end{align}
This ends the proof of the Reconstruction Theorem for \(\gamma \leq 0\). 